Fixed up multisubst

03Debruijn/Multisubst.thy
@@ -5,42 +5,57 @@ begin
 subsection \<open>Multiple substitution\<close>
 
 text \<open>We now want to prove termination. But in order to do that, we need one more tool. Multiple
-substitution replaces every free variable in an expression with a sequence of closed expressions.\<close>
+substitution replaces every free variable above an index in an expression with a sequence of closed 
+expressions. We will most often be using it with an index of 0, that is, eliminating _all_ free 
+variables. \<close>
 
-primrec multisubst :: "expr\<^sub>d list \<Rightarrow> expr\<^sub>d \<Rightarrow> expr\<^sub>d" where
-  "multisubst [] e = e"
-| "multisubst (e' # es) e = multisubst es (subst\<^sub>d 0 e' e)"
+primrec multisubst' :: "nat \<Rightarrow> expr\<^sub>d list \<Rightarrow> expr\<^sub>d \<Rightarrow> expr\<^sub>d" where
+  "multisubst' x [] e = e"
+| "multisubst' x (e' # es) e = multisubst' x es (subst\<^sub>d x e' e)"
 
-lemma multisubst_no_vars [simp]: "[] \<turnstile>\<^sub>d e : t \<Longrightarrow> multisubst es e = e"
+abbreviation multisubst :: "expr\<^sub>d list \<Rightarrow> expr\<^sub>d \<Rightarrow> expr\<^sub>d" where
+  "multisubst es e \<equiv> multisubst' 0 es e"
+
+lemma multisubst_no_vars [simp]: "[] \<turnstile>\<^sub>d e : t \<Longrightarrow> multisubst' x es e = e"
   by (induction es) simp_all
 
-text \<open>Explicitly multiple-substituting over constructors is easy in every case but one. Binders 
-cause problems for a simple compositional definition, because they increment the substitution index
-and \<open>multisubst\<close> only substitutes at 0. We provide a simple solution here and a more precise one, 
-using typechecking side conditions, below.\<close>
+lemma multisubst'_var1 [simp]: "x \<ge> y \<Longrightarrow> lookup vs (x - y) = Some v \<Longrightarrow> 
+  (\<And>v es. v \<in> set vs \<Longrightarrow> multisubst' y es v = v) \<Longrightarrow> multisubst' y vs (Var\<^sub>d x) = v"
+proof (induction vs x rule: lookup.induct)
+  case (3 a as x)
+  thus ?case
+  proof (cases "y = Suc x")
+    case False
+    with 3 have "Suc x - y = Suc (x - y)" by simp
+    with 3 False show ?thesis by simp
+  qed simp_all
+qed simp_all
 
-lemma multisubst_var [simp]: "lookup vs x = Some v \<Longrightarrow> 
+lemma multisubst_var1 [simp]: "lookup vs x = Some v \<Longrightarrow> 
     (\<And>v es. v \<in> set vs \<Longrightarrow> multisubst es v = v) \<Longrightarrow> multisubst vs (Var\<^sub>d x) = v"
-  by (induction vs x rule: lookup.induct) simp_all
+  by simp
 
-lemma multisubst_const [simp]: "multisubst es (Const\<^sub>d n) = Const\<^sub>d n"
+lemma multisubst_var2 [simp]: "x < y \<Longrightarrow> multisubst' y vs (Var\<^sub>d x) = Var\<^sub>d x"
+  by (induction vs) simp_all
+
+lemma multisubst_const [simp]: "multisubst' x es (Const\<^sub>d n) = Const\<^sub>d n"
   by (induction es) simp_all
 
-lemma multisubst_lam_simple [simp]: "\<exists>e'. multisubst es (Lam\<^sub>d t e) = Lam\<^sub>d t e'"
+lemma multisubst_lam [simp]: "multisubst' x es (Lam\<^sub>d t e) = 
+    Lam\<^sub>d t (multisubst' (Suc x) (map (incr\<^sub>d 0) es) e)"
   by (induction es arbitrary: e) simp_all
 
-lemma multisubst_app [simp]: "multisubst es (App\<^sub>d e\<^sub>1 e\<^sub>2) = App\<^sub>d (multisubst es e\<^sub>1) (multisubst es e\<^sub>2)"
+lemma multisubst_app [simp]: "multisubst' x es (App\<^sub>d e\<^sub>1 e\<^sub>2) = 
+    App\<^sub>d (multisubst' x es e\<^sub>1) (multisubst' x es e\<^sub>2)"
   by (induction es arbitrary: e\<^sub>1 e\<^sub>2) simp_all
 
-lemma multisubst_let_simple [simp]: "\<exists>e\<^sub>2'. multisubst es (Let\<^sub>d e\<^sub>1 e\<^sub>2) = Let\<^sub>d (multisubst es e\<^sub>1) e\<^sub>2'"
+lemma multisubst_let [simp]: "multisubst' x es (Let\<^sub>d e\<^sub>1 e\<^sub>2) = 
+    Let\<^sub>d (multisubst' x es e\<^sub>1) (multisubst' (Suc x) (map (incr\<^sub>d 0) es) e\<^sub>2)"
   by (induction es arbitrary: e\<^sub>1 e\<^sub>2) simp_all
 
-lemma multisubst_lam_to_app [dest]: "App\<^sub>d e\<^sub>1 e\<^sub>2 = multisubst es (Lam\<^sub>d t e) \<Longrightarrow> False"
-proof -
-  assume "App\<^sub>d e\<^sub>1 e\<^sub>2 = multisubst es (Lam\<^sub>d t e)"
-  moreover obtain e' where "multisubst es (Lam\<^sub>d t e) = Lam\<^sub>d t e'" by fastforce
-  ultimately show ?thesis by simp
-qed
+lemma multisubst_subst_swap: "y \<le> x \<Longrightarrow> multisubst' x es (subst\<^sub>d y e' e) = 
+    subst\<^sub>d y (multisubst' x es e') (multisubst' (Suc x) (map (incr\<^sub>d y) es) e)"
+  by (induction es arbitrary: e' e) simp_all
 
 text \<open>Typechecking the sequence of expressions to be multiply-substituted in is simple: they must 
 all be closed values, and they must match the typing context type-for-type. \<close>
@@ -50,6 +65,9 @@ inductive tc_expr_context :: "ty list \<Rightarrow> expr\<^sub>d list \<Rightarr
 | tcp_cons [simp]: "[] \<turnstile>\<^sub>d e : t \<Longrightarrow> value\<^sub>d e \<Longrightarrow> tc_expr_context \<Gamma> es \<Longrightarrow> 
     tc_expr_context (t # \<Gamma>) (e # es)"
 
+lemma tc_expr_context_incr [simp]: "tc_expr_context \<Gamma> es \<Longrightarrow> tc_expr_context \<Gamma> (map (incr\<^sub>d x) es)"
+  by (induction \<Gamma> es rule: tc_expr_context.induct) simp_all
+
 lemma tc_expr_context_insert [simp]: "tc_expr_context \<Gamma> es \<Longrightarrow> value\<^sub>d e \<Longrightarrow> x \<le> length \<Gamma> \<Longrightarrow> 
   [] \<turnstile>\<^sub>d e : t \<Longrightarrow> tc_expr_context (insert_at x t \<Gamma>) (insert_at x e es)"
 proof (induction \<Gamma> es arbitrary: x rule: tc_expr_context.induct)
@@ -57,35 +75,39 @@ proof (induction \<Gamma> es arbitrary: x rule: tc_expr_context.induct)
   then show ?case by (induction x) simp_all
 qed simp_all
 
-lemma tc_multisubst [simp]: "tc_expr_context \<Gamma> es \<Longrightarrow> \<Gamma> \<turnstile>\<^sub>d e : t \<Longrightarrow> [] \<turnstile>\<^sub>d multisubst es e : t"
+lemma tc_multisubst' [simp]: "tc_expr_context \<Gamma> es \<Longrightarrow> \<Gamma>' @ \<Gamma> \<turnstile>\<^sub>d e : t \<Longrightarrow> 
+  \<Gamma>' \<turnstile>\<^sub>d multisubst' (length \<Gamma>') es e : t"
 proof (induction \<Gamma> es arbitrary: e rule: tc_expr_context.induct)
   case (tcp_cons e' t' \<Gamma> es)
-  moreover hence "insert_at 0 t' \<Gamma> \<turnstile>\<^sub>d e : t" by (induction \<Gamma>) simp_all
-  moreover from tcp_cons have "[] \<turnstile>\<^sub>d e' : t'" by simp
-  moreover hence "\<Gamma> \<turnstile>\<^sub>d e' : t'" using tc_postpend by fastforce
-  ultimately show ?case by simp
+  hence "\<Gamma>' @ \<Gamma> \<turnstile>\<^sub>d e' : t'" by (metis append_Nil tc_postpend)
+  with tcp_cons show ?case by simp
 qed simp_all
 
-lemma multisubst_lam_complex [simp]: "tc_expr_context \<Gamma> es \<Longrightarrow> insert_at 0 t\<^sub>1 \<Gamma> \<turnstile>\<^sub>d e : t\<^sub>2 \<Longrightarrow> 
-  \<exists>e'. multisubst es (Lam\<^sub>d t\<^sub>1 e) = Lam\<^sub>d t\<^sub>1 e' \<and> ([t\<^sub>1] \<turnstile>\<^sub>d e' : t\<^sub>2) \<and>
-    (\<forall>e\<^sub>2. ([] \<turnstile>\<^sub>d e\<^sub>2 : t\<^sub>1) \<longrightarrow> multisubst es (subst\<^sub>d 0 e\<^sub>2 e) = subst\<^sub>d 0 e\<^sub>2 e')"
+lemma tc_multisubst [simp]: "tc_expr_context \<Gamma> es \<Longrightarrow> \<Gamma> \<turnstile>\<^sub>d e : t \<Longrightarrow> [] \<turnstile>\<^sub>d multisubst es e : t"
+proof -
+  assume "\<Gamma> \<turnstile>\<^sub>d e : t" 
+  hence "[] @ \<Gamma> \<turnstile>\<^sub>d e : t" by simp
+  moreover assume "tc_expr_context \<Gamma> es"
+  ultimately show ?thesis using tc_multisubst' by fastforce
+qed
+
+lemma multisubst_above [simp]: "\<Gamma> \<turnstile>\<^sub>d e : t \<Longrightarrow> multisubst' (length \<Gamma>) es e = e"
+  by (induction es) simp_all
+
+lemma multisubst_twice [simp]: "tc_expr_context \<Gamma> es \<Longrightarrow> \<Gamma>' @ \<Gamma> \<turnstile>\<^sub>d e : t \<Longrightarrow> 
+    multisubst' (length \<Gamma>') es' (multisubst' (length \<Gamma>') es e) = multisubst' (length \<Gamma>') es e"
+proof -
+  assume "tc_expr_context \<Gamma> es" and "\<Gamma>' @ \<Gamma> \<turnstile>\<^sub>d e : t"
+  hence "\<Gamma>' \<turnstile>\<^sub>d multisubst' (length \<Gamma>') es e : t" by simp
+  thus ?thesis by simp
+qed
+
+lemma incr_multisubst_absorb [simp]: "tc_expr_context \<Gamma> es \<Longrightarrow> \<Gamma>' @ \<Gamma> \<turnstile>\<^sub>d e : t \<Longrightarrow> 
+  x \<ge> length \<Gamma>' \<Longrightarrow> incr\<^sub>d x (multisubst' (length \<Gamma>') es e) = multisubst' (length \<Gamma>') es e"
 proof (induction \<Gamma> es arbitrary: e rule: tc_expr_context.induct)
-  case (tcp_cons e' t \<Gamma> es)
-  hence "[] \<turnstile>\<^sub>d e' : t" by simp
-  hence "\<Gamma> \<turnstile>\<^sub>d e' : t" using tc_postpend by fastforce
-  hence "insert_at 0 t\<^sub>1 \<Gamma> \<turnstile>\<^sub>d incr\<^sub>d 0 e' : t" by simp
-  with tcp_cons show ?case by (cases \<Gamma>) simp_all
-qed simp_all
-
-lemma multisubst_let_complex [simp]: "tc_expr_context \<Gamma> es \<Longrightarrow> insert_at 0 t\<^sub>1 \<Gamma> \<turnstile>\<^sub>d e\<^sub>2 : t\<^sub>2 \<Longrightarrow> 
-  \<exists>e\<^sub>2'. multisubst es (Let\<^sub>d e\<^sub>1 e\<^sub>2) = Let\<^sub>d (multisubst es e\<^sub>1) e\<^sub>2' \<and> ([t\<^sub>1] \<turnstile>\<^sub>d e\<^sub>2' : t\<^sub>2) \<and>
-    (\<forall>v\<^sub>1. ([] \<turnstile>\<^sub>d v\<^sub>1 : t\<^sub>1) \<longrightarrow> multisubst es (subst\<^sub>d 0 v\<^sub>1 e\<^sub>2) = subst\<^sub>d 0 v\<^sub>1 e\<^sub>2')"
-proof (induction \<Gamma> es arbitrary: e\<^sub>1 e\<^sub>2 rule: tc_expr_context.induct)
-  case (tcp_cons e' t \<Gamma> es)
-  hence "[] \<turnstile>\<^sub>d e' : t" by simp
-  hence "\<Gamma> \<turnstile>\<^sub>d e' : t" using tc_postpend by fastforce
-  hence "insert_at 0 t\<^sub>1 \<Gamma> \<turnstile>\<^sub>d incr\<^sub>d 0 e' : t" by simp
-  with tcp_cons show ?case by (cases \<Gamma>) simp_all
+  case (tcp_cons e' t' \<Gamma> es)
+  moreover hence "\<Gamma>' @ \<Gamma> \<turnstile>\<^sub>d e' : t'" by (metis append.left_neutral tc_postpend)
+  ultimately show ?case by simp
 qed simp_all
 
 end
